examples/dm4all/IOFr2.fst
@@ -26,9 +26,11 @@ let rec bind (a : Type u#aa) (b : Type u#bb)
   | Write o k' -> Write o (bind _ _ k' k)
   | Return v -> k v
 
+unfold
 let return_wp (a:Type) (x:a) : wpty a =
   fun p -> p (x, [])
 
+unfold
 let bind_wp (_ : range) (a:Type) (b:Type) (w : wpty a) (kw : a -> wpty b) : wpty b =
   fun p -> w (fun (x, l1) -> kw x (fun (y, l2) -> p (y, l1 @ l2)))
   
@@ -69,16 +71,13 @@ let test1 () =
   write 3;
   1
   
-open FStar.Tactics
-
-(* GM: For some reason I need to compute() in order to prove this *)
-let test2 () : IO int (fun p -> p (1, [2; 3])) by (compute ()) =
+let test2 () : IO int (fun p -> p (1, [2; 3])) =
   write 2;
   let x = read () in
   write 3;
   1
 
-let test3 () : IO int (fun p -> forall x. p (1, [2; x])) by (compute ()) =
+let test3 () : IO int (fun p -> forall x. p (1, [2; x])) =
   write 2;
   let x = read () in
   let x = read () in
@@ -88,7 +87,7 @@ let test3 () : IO int (fun p -> forall x. p (1, [2; x])) by (compute ()) =
   1
 
 [@expect_failure]
-let test4 () : IO int (fun p -> forall x. p (1, [x; x])) by (compute ()) =
+let test4 () : IO int (fun p -> forall x. p (1, [x; x])) =
   write 2;
   let x = read () in
   let x = read () in
@@ -97,7 +96,7 @@ let test4 () : IO int (fun p -> forall x. p (1, [x; x])) by (compute ()) =
   write x;
   1
 
-let test5 () : IO int (fun p -> forall x. p (1, [x; x])) by (compute ()) =
+let test5 () : IO int (fun p -> forall x. p (1, [x; x])) =
   let x = read () in
   write x;
   write x;
